Splinter/Betree/PivotBetree.i.dfy
@@ -165,18 +165,6 @@ module PivotBetree
       if Nil? then [] else children
     }
 
-    predicate EquivalentBufferCompaction(other: BetreeNode)
-    {
-      && WF()
-      && other.WF()
-      && BetreeNode?
-      && other.BetreeNode?
-      && Buffers().Equivalent(other.Buffers())
-      // Can only make a local change; entirety of children subtrees are identical.
-      && pivotTable == other.pivotTable
-      && Children() == other.Children()
-    }
-
     predicate KeyInDomain(key: Key)
     {
       && WF()
@@ -446,18 +434,21 @@ module PivotBetree
       )
   }
 
-  // NB we tell you exactly how to Split and Flush, but leave lots of
-  // nondetermistic freedom in the description of Compact.
+  function CompactedNode(original: BetreeNode, newBufs: BufferStack) : BetreeNode 
+    requires original.BetreeNode?
+    requires original.buffers.Equivalent(newBufs)
+  {
+    BetreeNode(newBufs, original.pivotTable, original.children)
+  }
+
   predicate InternalCompact(v: Variables, v': Variables, lbl: TransitionLabel, step: Step)
+    requires step.WF()
   {
     && lbl.InternalLabel?
     && step.InternalCompactStep?
-    && step.path.Valid()
     && step.path.node == v.root
-    && step.compactedNode.WF()
-    && step.path.Target().EquivalentBufferCompaction(step.compactedNode)
     && v' == v.(
-          root := step.path.Substitute(step.compactedNode)
+          root := step.path.Substitute(CompactedNode(step.path.Target(), step.compactedBuffers))
       )
   }
 
@@ -477,7 +468,7 @@ module PivotBetree
     | InternalGrowStep()
     | InternalSplitStep(path: Path, childIdx: nat, splitKey: Key)
     | InternalFlushStep(path: Path, childIdx: nat)
-    | InternalCompactStep(path: Path, compactedNode: BetreeNode)
+    | InternalCompactStep(path: Path, compactedBuffers: BufferStack)
   {
     predicate WF() {
       match this {
@@ -489,9 +480,10 @@ module PivotBetree
         case InternalFlushStep(path, childIdx) =>
           && path.Valid()
           && path.Target().ValidChildIndex(childIdx)
-        case InternalCompactStep(path, compactedNode) =>
+        case InternalCompactStep(path, compactedBuffers) =>
           && path.Valid()
-          && compactedNode.WF()
+          && path.Target().BetreeNode?  // no point compacting a nil node
+          && path.Target().buffers.Equivalent(compactedBuffers)
         case _ => true
       }
     }
@@ -499,16 +491,17 @@ module PivotBetree
 
   predicate NextStep(v: Variables, v': Variables, lbl: TransitionLabel, step: Step)
   {
-    match step {
-      case QueryStep(receipt) => Query(v, v', lbl, receipt)
-      case PutStep() => Put(v, v', lbl)
-      case QueryEndLsnStep() => QueryEndLsn(v, v', lbl)
-      case FreezeAsStep() => FreezeAs(v, v', lbl)
-      case InternalGrowStep() => InternalGrow(v, v', lbl, step)
-      case InternalSplitStep(_, _, _) => InternalSplit(v, v', lbl, step)
-      case InternalFlushStep(_, _) => InternalFlush(v, v', lbl, step)
-      case InternalCompactStep(_, _) => InternalCompact(v, v', lbl, step)
-    }
+    && step.WF()
+    && match step {
+        case QueryStep(receipt) => Query(v, v', lbl, receipt)
+        case PutStep() => Put(v, v', lbl)
+        case QueryEndLsnStep() => QueryEndLsn(v, v', lbl)
+        case FreezeAsStep() => FreezeAs(v, v', lbl)
+        case InternalGrowStep() => InternalGrow(v, v', lbl, step)
+        case InternalSplitStep(_, _, _) => InternalSplit(v, v', lbl, step)
+        case InternalFlushStep(_, _) => InternalFlush(v, v', lbl, step)
+        case InternalCompactStep(_, _) => InternalCompact(v, v', lbl, step)
+      }
   }
 
   predicate Next(v: Variables, v': Variables, lbl: TransitionLabel) {
